Pauline/Interp.lean
@@ -1,0 +1,127 @@
+import Std
+import Pauline.Dynamics
+
+open Std
+
+/- This is poorly implemented, probably should be rewritten -/
+namespace Pauline
+
+open Dynamic
+
+inductive StepRes (init : State × Exp)
+  | val   : isVal init.2 → StepRes init
+  | var   : Ident → StepRes init -- free variable
+  | raise : Ident → StepRes init
+  | step  : (s : State) → (e : Exp) → StepExp init (s, e) → StepRes init
+
+def StepRes.toString : StepRes init → String
+  | .val _ => "val"
+  | .var x => s!"free-var: {x}"
+  | .raise x => s!"raise {x}"
+  | .step _s' e' _h => s!"stepped: {e'}"
+instance : ToString (StepRes init) := ⟨StepRes.toString⟩
+
+/- should require `e` typechecks rather than basically dynamically checking -/
+def step (s : State) (exp : Exp) : StepRes (s, exp) :=
+  match hexp : exp with
+  | .scon sc  => .val (by simp [isVal])
+  | .var x    =>
+    match h : s.find x with
+    | some e => .step s e.val (.varStep h)
+    | none   => .var x
+  | .tuple [] => .val (by simp [isVal])
+  | .tuple (e :: es) =>
+    match step s e with
+    | .val he =>
+      match step s (.tuple es) with
+      | .val hes => .val (by simp [isVal]; exact ⟨he, hes⟩)
+      | .var x => .var x
+      | .raise exn => .raise exn
+      | .step s' (.tuple es') hes =>
+        .step s' (.tuple (e::es')) (.tupleTlStep he sorry hes)
+    | .var x => .var x
+    | .raise exn => .raise exn
+    | .step s' e' he => .step s' (.tuple (e'::es)) (.tupleHdStep (sorry) he)
+  | .raise e =>
+    match step s e with
+    | .var x => .var x
+    | .raise exn => .raise exn
+    | .step s' e' h => .step s' (.raise e') (.raiseStep h)
+    | _ => .raise "INVALID"
+  | .let_in _ _ => .raise "FAIL: Implement"
+  | .app f e =>
+    match step s f with
+    | .step s' f' h => .step s' (.app f' e) (.appStepL (sorry) h)
+    | .raise exn    => .raise exn
+    | .var x        => .var x
+    | .val hf        =>
+      match step s e with
+      | .step s' e' he => .step s' (.app f e') (.appStepR hf he)
+      | .raise exn     => .raise exn
+      | .var x         => .var x
+      | .val he =>
+          match f with
+          | .lam p body =>
+            .step s (substPat body ⟨e, he⟩ p) (.appStep he rfl)
+          | .extern _ exe =>
+            .step s (callExtern exe ⟨e, he⟩) (.externStep he rfl)
+          | _ => .raise s!"FAIL: SOMETHING WENT WRONG {Exp.app f e}"
+  | .typed e τ => .step s e .typedStep
+  | .ite b t f =>
+    match b with
+    | .scon (.bool true)  => .step s t (.iteStepT rfl)
+    | .scon (.bool false) => .step s f (.iteStepF rfl)
+    | _ =>
+      match step s b with
+      | .step s' b' h => .step s' (.ite b' t f) (.iteStepB sorry)
+      | .var x => .var x
+      | .raise exn => .raise exn
+      | _ => .raise s!"FAIL: SOMETHING WENT WRONG ITE {b}"
+  | .case e cl => .raise "FAIL: Implement"
+  | .lam p body => .val (by simp [isVal])
+  | .extern _ exe => .val (by simp [isVal])
+
+inductive EvalRes (init : State × Exp)
+| val : (e : {e // isVal e}) → StepsExp init (s, e.val) → EvalRes init
+| var : Ident → StepsExp init (s, e) → EvalRes init
+| raise : Ident → StepsExp init (s, e) → EvalRes init
+| nop : StepsExp init init → EvalRes init
+
+instance : Inhabited (EvalRes init) where
+  default := .nop ⟨0, by simp [StepsNExp]⟩
+
+def EvalRes.exp : EvalRes init → Exp
+  | .val e _            => e.val
+  | .var (e := e) _ _   => e
+  | .raise (e := e) _ _ => e
+  | .nop _              => init.2
+
+def EvalRes.state : EvalRes init → State
+  | .val (s := s) _ _   => s
+  | .var (s := s) _ _   => s
+  | .raise (s := s) _ _ => s
+  | .nop _              => init.1
+
+def EvalRes.property : (res : EvalRes init) → StepsExp init (res.state, res.exp)
+  | .val _ h   => h
+  | .var _ h   => h
+  | .raise _ h => h
+  | .nop h     => h
+
+def EvalRes.toString : EvalRes init → String
+  | .val e _ => s!"val {e.val}"
+  | .var (e:=e) x _ => s!"free-var: {x} in {e}"
+  | .raise x _ => s!"raise {x}"
+  | .nop _   => "nop"
+instance : ToString (EvalRes init) := ⟨EvalRes.toString⟩
+
+partial def eval_acc (s : State) (e : Exp) (acc : StepsExp init (s, e))
+    : EvalRes init  :=
+  match step s e with
+  | .step s' e' h => eval_acc s' e' (trans acc h)
+  | .val h => .val ⟨e, h⟩ acc
+  | .var x => .var x acc
+  | .raise exn => .raise exn acc
+
+def eval (s : State) (e : Exp) : EvalRes (s, e) :=
+  eval_acc s e (⟨0, by simp [StepsNExp]⟩)
